messageInvariantPrototypes/paxos/automate_full/applicationProof.dfy
@@ -1012,7 +1012,6 @@ returns (accSet: set<AcceptorId>)
   ensures forall a :: c.ValidAcceptorIdx(a) <==> a in accSet
   ensures |accSet| == 2 * c.f + 1
 {
-  assert v.History(0).WF(c);  // trigger for |c.acceptors| == 2 * c.f+1
   accSet := set a |  0 <= a < |c.acceptors|;
   SetComprehensionSize(|c.acceptors|);
 }
